modify jit flattern

theory/JITFlattern.thy
@@ -37,7 +37,16 @@ lemma list_in_list_prop1:"list_in_list l2 (length l1) (l1@l2@l3) \<Longrightarro
   list_in_list l2 (length l1+length l1') (l1'@((l1@l2@l3))@l3')"
   sorry*)
 
-lemma list_in_list_prop2:"list_in_list l xpc l_bin \<Longrightarrow> x64_decode 0 l = x64_decode xpc l_bin"
+(*lemma "list_in_list l xpc l_bin \<Longrightarrow> length l = len \<Longrightarrow> l  \<noteq> [] \<Longrightarrow> 
+  idx \<ge>0 \<and> idx < len \<Longrightarrow> l!idx = l_bin!(xpc+idx)"
+  apply(induction l arbitrary:xpc l_bin len idx)
+   apply simp
+  subgoal for a l xpc l_bin len idx 
+    sorry
+  done
+*)
+
+lemma list_in_list_prop2:"list_in_list l xpc l_bin \<Longrightarrow> x64_decode x l = x64_decode (xpc+x) l_bin"
   sorry
 
 
@@ -206,21 +215,23 @@ lemma flattern_l_bin0:
 
 lemma flattern_num_easy:
   "l_bin0!(unat pc)=(num,off,l) \<Longrightarrow>
-  l_bin0 \<noteq> [] \<and> unat pc < length l \<and> unat pc \<ge> 0 \<Longrightarrow>
-  jitflat_bpf l_bin0 init_second_layer = (l2,l_pc2,l_jump2) \<Longrightarrow>
-  snd (l_pc2!(unat pc)) = num"
+   unat pc < length l_bin0 \<and> unat pc \<ge> 0 \<Longrightarrow>
+   jitflat_bpf l_bin0 init_second_layer = (l2,l_pc2,l_jump2) \<Longrightarrow>
+   snd (l_pc2!(unat pc)) = num"
 proof(induct l_bin0 arbitrary: pc num off l l2 l_pc2 l_jump2)
-  case Nil
-  then show ?case by blast
+  case Nil 
+  have "length l_bin0 = 0" using Nil by simp
+  then show ?case using Nil.prems(2) by auto  
+    
 next
   case (Cons a l_bin0)
   then show ?case
   proof-
   have assm1:"(a # l_bin0) ! unat pc = (num, off, l)" using Cons by simp
-  have assm2:"a # l_bin0 \<noteq> [] \<and> unat pc < length l \<and> (0::nat) \<le> unat pc" using Cons by simp
+  have assm2:"unat pc < length (a # l_bin0) \<and> (0::nat) \<le> unat pc" using Cons by simp
   have assm3:"jitflat_bpf (a # l_bin0) init_second_layer = (l2, l_pc2, l_jump2)" using Cons by simp
   
-  have "l_bin0 ! unat pc = (num, off, l) \<Longrightarrow> l_bin0 \<noteq> [] \<and> unat pc < length l \<and> (0::nat) \<le> unat pc \<Longrightarrow>
+  have "l_bin0 ! unat pc = (num, off, l) \<Longrightarrow> unat pc < length l_bin0 \<and> (0::nat) \<le> unat pc \<Longrightarrow>
     jitflat_bpf l_bin0 init_second_layer = (l2, l_pc2, l_jump2) \<Longrightarrow> snd (l_pc2 ! unat pc) = num"
     using Cons by simp
 
@@ -228,63 +239,66 @@ next
   show ?thesis
   proof(cases "unat pc = 0")
     case True
-    let "?x" = "tl l_bin0"
-
-    have "snd (l_pc2!(unat pc)) = num" using not_change_prefix_l_pc True
-      by (smt (verit, ccfv_threshold) append_Nil assm1 assm3 init_second_layer_def jitflat_bpf.simps(2) list_in_list.simps(2) nth_Cons_0 prod.collapse prod.inject)
-    then show ?thesis by simp
+      let "?x" = "tl l_bin0"
+  
+      have "snd (l_pc2!(unat pc)) = num" using not_change_prefix_l_pc True
+        by (smt (verit, ccfv_threshold) append_Nil assm1 assm3 init_second_layer_def jitflat_bpf.simps(2) list_in_list.simps(2) nth_Cons_0 prod.collapse prod.inject)
+      then show ?thesis by simp
   next
     case False
-    have b0:"unat pc \<ge>1" using False a0 by simp
-    let "?pc" = "unat pc -1"
-    have b1:"?pc < length l \<and> (0::nat) \<le> ?pc" using assm2 b0 using diff_le_self order_le_less_trans by blast 
-    let "?x" = "tl l_bin0"
-    have b2:"l_bin0 ! ?pc = (num, off, l)" using assm1
-      by (simp add: False order_neq_le_trans) 
-    
-    have b2_1:"jitflat_bpf (a#l_bin0) init_second_layer = (
-      jitflat_bpf l_bin0 (
-        []@(snd(snd a)),
-        []@[(0, fst a)],
-        update_l_jump a [] []))" using init_second_layer_def 
-      by (metis jitflat_bpf.simps(2) list.size(3) prod.exhaust_sel semiring_1_class.of_nat_0) 
-
-    hence b2_2:"jitflat_bpf (a#l_bin0) init_second_layer = jitflat_bpf l_bin0 ((snd(snd a)),[(0, fst a)],update_l_jump a [] [])" by auto
-    
-    have "\<exists> l2' l_pc2' l_jump2'. jitflat_bpf l_bin0 init_second_layer = (l2',l_pc2',l_jump2') " by (metis surj_pair)
-    then obtain l2' l_pc2' l_jump2' where b3_1:"jitflat_bpf l_bin0 init_second_layer = (l2',l_pc2',l_jump2')" by auto
-    have b4:"l_bin0 \<noteq> []" sorry
-    have b3:"snd (l_pc2'! ?pc) = num" using Cons False using b0 b1 b2 b3_1 b4
-      by (metis (mono_tags, lifting) order_neq_le_trans unat_gt_0 unat_minus_one) 
-
-    have c0:"map snd l_pc2' = map fst l_bin0" using num_corr b3_1 init_second_layer_def
-      by (metis append_Nil append_eq_conv_conj) 
-    have c1:"map snd l_pc2 = map fst (a#l_bin0)" using num_corr assm3 init_second_layer_def
-      by (metis drop0 list.size(3)) 
-    (*have c2:"l_pc2 \<noteq> []" using c1 by auto
-    have c3:"l_pc2' \<noteq> []" sorry*)
-    (*have c2:"map fst (a#l_bin0) = fst a # map fst l_bin0" by auto*)
-
-    (*have "\<exists> l2'' l_pc2'' l_jump2''. jitflat_bpf [a] init_second_layer = l2'' l_pc2'' l_jump2''" by blast
-    then obtain l2'' l_pc2'' l_jump2'' where "jitflat_bpf [a] init_second_layer = l2'' l_pc2'' l_jump2''" by auto
-    have b2_3:"list_in_list [(0, fst a)] 0 l_pc2" using not_change_prefix_l_pc b2_2 assm3 by metis
-    have b2_4:"l_pc2!0 = (0, fst a)" using b2_3 by auto*)
-    have "map snd l_pc2 = (fst a)#(map snd l_pc2')" using c0 c1 b2_2 by auto
-      (*using assm3 b3 init_second_layer_def not_change_prefix_l_pc b2_2 b2_3 b2_4 num_corr *)
-    hence "(map snd l_pc2)!(unat pc) = (map snd l_pc2')!?pc" using b3 False by auto
-    hence "snd (l_pc2! unat pc) = num" using b3 False order_neq_le_trans sorry
-    then show ?thesis by auto  
+      have b0:"unat pc \<ge>1" using False a0 by simp
+      let "?pc" = "unat pc -1"
+      have b1:"?pc < length l_bin0 \<and> (0::nat) \<le> ?pc" using assm2 b0 using diff_le_self order_le_less_trans by simp
+      let "?x" = "tl l_bin0"
+      have b2:"l_bin0 ! ?pc = (num, off, l)" using assm1
+        by (simp add: False order_neq_le_trans) 
+      
+      have b2_1:"jitflat_bpf (a#l_bin0) init_second_layer = (
+        jitflat_bpf l_bin0 (
+          []@(snd(snd a)),
+          []@[(0, fst a)],
+          update_l_jump a [] []))" using init_second_layer_def 
+        by (metis jitflat_bpf.simps(2) list.size(3) prod.exhaust_sel semiring_1_class.of_nat_0) 
+  
+      hence b2_2:"jitflat_bpf (a#l_bin0) init_second_layer = jitflat_bpf l_bin0 ((snd(snd a)),[(0, fst a)],update_l_jump a [] [])" by auto
+      
+      have "\<exists> l2' l_pc2' l_jump2'. jitflat_bpf l_bin0 init_second_layer = (l2',l_pc2',l_jump2') " by (metis surj_pair)
+      then obtain l2' l_pc2' l_jump2' where b3_1:"jitflat_bpf l_bin0 init_second_layer = (l2',l_pc2',l_jump2')" by auto
+      (*have b4:"l_bin0 \<noteq> []" sorry*)
+  
+        have b3:"snd (l_pc2'! ?pc) = num" using Cons False using b0 b1 b2 b3_1 
+        by (metis (mono_tags, lifting) order_neq_le_trans unat_gt_0 unat_minus_one) 
+  
+      have c0:"map snd l_pc2' = map fst l_bin0" using num_corr b3_1 init_second_layer_def
+        by (metis append_Nil append_eq_conv_conj) 
+      have c1:"map snd l_pc2 = map fst (a#l_bin0)" using num_corr assm3 init_second_layer_def
+        by (metis drop0 list.size(3)) 
+      (*have c2:"l_pc2 \<noteq> []" using c1 by auto
+      have c3:"l_pc2' \<noteq> []" sorry*)
+      (*have c2:"map fst (a#l_bin0) = fst a # map fst l_bin0" by auto*)
+  
+      (*have "\<exists> l2'' l_pc2'' l_jump2''. jitflat_bpf [a] init_second_layer = l2'' l_pc2'' l_jump2''" by blast
+      then obtain l2'' l_pc2'' l_jump2'' where "jitflat_bpf [a] init_second_layer = l2'' l_pc2'' l_jump2''" by auto
+      have b2_3:"list_in_list [(0, fst a)] 0 l_pc2" using not_change_prefix_l_pc b2_2 assm3 by metis
+      have b2_4:"l_pc2!0 = (0, fst a)" using b2_3 by auto*)
+      have "map snd l_pc2 = (fst a)#(map snd l_pc2')" using c0 c1 b2_2 by auto
+        (*using assm3 b3 init_second_layer_def not_change_prefix_l_pc b2_2 b2_3 b2_4 num_corr *)
+      hence "(map snd l_pc2)!(unat pc) = (map snd l_pc2')!?pc" using b3 False by auto
+      hence "snd (l_pc2! unat pc) = num" 
+        using b3 False by (metis assm2 b1 c0 c1 map_equality_iff nth_map)
+      then show ?thesis by auto  
+    qed
   qed
 qed
-qed
 
-
+(*
 lemma flattern_num:
   assumes a0:"l_bin0!(unat pc)=(num,off,l)" and
    a1:"l_pc2 \<noteq> []" and
-   a2:"jitflat_bpf l_bin0 (l1,l_pc1,l_jump1) = (l2,l_pc2,l_jump2)"
+   a2:"jitflat_bpf l_bin0 (l1,l_pc1,l_jump1) = (l2,l_pc2,l_jump2)" and
+   a3:"unat pc < length l_bin0 \<and> unat pc \<ge> 0"
  shows "snd (l_pc2!(length l_pc1 + unat pc)) = num"
-  sorry
+  sorry*)
 
 fun find_target_pc_in_l_pc :: "((u64\<times>u64) list) \<Rightarrow> u64 \<Rightarrow> u64 option" where
 "find_target_pc_in_l_pc [] _ = None" |
@@ -328,14 +342,206 @@ fun flat_bpf_sem :: "nat \<Rightarrow> flat_bpf_prog \<Rightarrow> hybrid_state 
 )"
 
 
+definition match_state1::"outcome \<Rightarrow> outcome \<Rightarrow> bool" where
+  "match_state1 fxst xxst \<equiv> 
+  (case fxst of (Next xst xrs xm xss) \<Rightarrow>
+    (case xxst of (Next xst1 xrs1 xm1 xss1) \<Rightarrow> 
+     xrs = xrs1 \<and> xm = xm1 \<and> xss = xss1 |
+                   _ \<Rightarrow> False)|
+                 _ \<Rightarrow> False)"
+
+definition match_state::"hybrid_state \<Rightarrow> hybrid_state \<Rightarrow> bool" where
+  "match_state fxst xxst \<equiv> 
+  (case fxst of (pc,Next xst xrs xm xss) \<Rightarrow>
+    (case xxst of (pc1,Next xst1 xrs1 xm1 xss1) \<Rightarrow> 
+      pc = pc1 \<and> match_state1 (Next xst1 xrs1 xm1 xss1) (Next xst xrs xm xss)  |
+                   _ \<Rightarrow> False)|
+                 _ \<Rightarrow> False)"
+(*x64_decode 0 l = x64_decode xpc l
+xxst = Next xpc1 xrs1 xm1 xss1 \<Longrightarrow>
+   fxst = Next xpc2 xrs2 xm2 xss2 \<Longrightarrow>
+xrs1 = xrs2 \<and> xm1 = xm2 \<and> xss1 = xss2*)
+
+lemma err_is_still_err2:"x64_sem n l Stuck = xst' \<Longrightarrow> xst' = Stuck "
+  apply(induct n, simp)
+  using perir_step_def
+  by auto
+
+lemma intermediate_step_is_ok2:
+  "x64_sem n l xst = xst' \<Longrightarrow> n \<ge> 0 \<Longrightarrow> xst' \<noteq> Stuck \<Longrightarrow> \<exists> xpc xrs xm xss. xst = (Next xpc xrs xm xss)"
+  apply(induct n arbitrary: l xst xst')
+   apply simp apply (meson outcome.exhaust) 
+  using err_is_still_err2 by (metis outcome.exhaust)
+
+lemma list_in_list_prop3:"x64_sem num l_bin (Next (xpc+x) xrs xm xss) = fxst \<Longrightarrow>
+   x64_sem num l (Next x xrs xm xss) = xxst \<Longrightarrow>
+   list_in_list l xpc l_bin \<Longrightarrow>
+   xxst \<noteq> Stuck \<Longrightarrow>
+   match_state1 xxst fxst"
+proof(induction num arbitrary:l_bin xpc x xrs xm xss fxst l xrs xm xss xxst)
+  case 0
+  then show ?case using match_state1_def by auto
+next
+  case (Suc num)
+  assume assm0:"x64_sem (Suc num) l_bin (Next (xpc+x) xrs xm xss) = fxst" and
+      assm1:"x64_sem (Suc num) l (Next x xrs xm xss) = xxst" and
+      assm2:"list_in_list l xpc l_bin" and
+      assm3:"xxst \<noteq> Stuck"
+
+  have "x64_sem 1 l_bin (Next (xpc+x) xrs xm xss) = 
+              (case x64_decode (xpc+x) l_bin of
+                None \<Rightarrow> Stuck |
+                Some (sz, ins) \<Rightarrow>
+             x64_sem 0 l_bin (exec_instr ins sz (xpc+x) xrs xm xss))" by simp
+  hence b0:"x64_sem 1 l_bin (Next (xpc+x) xrs xm xss) = 
+              (case x64_decode (xpc+x) l_bin of
+                None \<Rightarrow> Stuck |
+                Some (sz, ins) \<Rightarrow>
+             (exec_instr ins sz (xpc+x) xrs xm xss))"
+    using x64_sem.simps(1) by presburger 
+
+  have "x64_sem 1 l (Next x xrs xm xss) = 
+              (case x64_decode x l of
+                None \<Rightarrow> Stuck |
+                Some (sz, ins) \<Rightarrow>
+             x64_sem 0 l (exec_instr ins sz x xrs xm xss))" by simp
+  hence d0:"x64_sem 1 l (Next x xrs xm xss) = 
+              (case x64_decode x l of
+                None \<Rightarrow> Stuck |
+                Some (sz, ins) \<Rightarrow>
+             (exec_instr ins sz x xrs xm xss))"
+    using x64_sem.simps(1) by presburger  
+  have a0:"x64_decode x l = x64_decode (xpc+x) l_bin" using assm2 list_in_list_prop2
+    by (metis add_0 list_in_list.simps(1))
+
+
+  have d1_0:"x64_sem 1 l (Next x xrs xm xss) \<noteq> Stuck" 
+    using assm3 assm1 by (metis err_is_still_err2 plus_1_eq_Suc x64_sem_add) 
+  hence d1_1:"x64_decode x l \<noteq> None" using d0 by(cases "x64_decode x l",simp_all)
+  hence "\<exists> sz ins. x64_decode x l = Some (sz,ins)" by simp
+  then obtain sz ins where d1_2:"x64_decode x l = Some (sz,ins)" by auto
+  hence d1:"x64_sem 1 l (Next x xrs xm xss) = (exec_instr ins sz x xrs xm xss)" 
+    using d0 by fastforce 
+
+  hence "\<exists> xpc'' xrs'' xm'' xss''. exec_instr ins sz x xrs xm xss = Next xpc'' xrs'' xm'' xss''" 
+    using d1 outcome.exhaust d1_0 by metis
+  then obtain xpc'' xrs'' xm'' xss'' where d2:"exec_instr ins sz x xrs xm xss = Next xpc'' xrs'' xm'' xss''" by auto
+
+  have b1:"x64_sem 1 l_bin (Next (xpc+x) xrs xm xss) = (exec_instr ins sz (xpc+x) xrs xm xss)"
+    using d1_1 d1_2 b0 a0 by simp
+  (* have "x64_sem 1 l_bin (Next (xpc+x) xrs xm xss) \<noteq> Stuck" using intermediate_step_is_ok2 sorry*)
+  thus ?case
+  proof(cases "x64_sem 1 l_bin (Next (xpc+x) xrs xm xss) \<noteq> Stuck")
+    case True
+    hence "\<exists> xpc' xrs' xm' xss'. exec_instr ins sz (xpc+x) xrs xm xss = Next xpc' xrs' xm' xss'"
+       using b1 outcome.exhaust by metis
+    then obtain xpc' xrs' xm' xss' where b2:"exec_instr ins sz (xpc+x) xrs xm xss = Next xpc' xrs' xm' xss'" by auto
+            (*xpc' = xpc1 + sz \<and> xpc'' = 0 + sz \<and> *)
+    have a1:"xrs'' = xrs' \<and> xm'' = xm' \<and> xss'' = xss'"
+              using b2 d2 apply(unfold exec_instr_def)
+              apply(cases ins,simp_all)
+              subgoal for x7 apply(unfold exec_push_def Let_def)
+                apply(cases "storev M64 xm (Vptr sp_block (xrs (IR SP) - u64_of_memory_chunk M64)) (Vlong (xrs (IR x7)))",simp_all)
+                done
+              subgoal for x8 apply(unfold exec_pop_def Let_def)
+                apply(cases "loadv M64 xm (Vptr sp_block (xrs (IR SP)))",simp_all)
+                subgoal for a apply(cases a,simp_all)
+                  done
+                done
+              subgoal for x131 x132 apply(cases "eval_testcond x131 xrs",simp_all)
+                subgoal for a 
+                  by (metis outcome.inject) 
+                done
+              subgoal for x151 x152 x153
+                apply(unfold exec_store_def,simp_all)
+                apply(cases "storev x153 xm (Vlong (eval_addrmode64 x151 xrs)) (Vlong (xrs (IR x152)))",simp_all)
+                done
+              subgoal for x201 x202 x203 
+                apply(unfold exec_load_def,simp_all)
+                apply(cases "loadv x203 xm (Vlong (eval_addrmode64 x202 xrs))",simp_all)
+                subgoal for a apply(cases a,simp_all)
+                  done
+                done
+              subgoal for x21a 
+                apply(unfold exec_call_def,simp_all)
+                done
+              done
+    have a2:"xpc'' = x + sz \<and> xpc'= xpc + x + sz" sorry
+  
+    let "?x" = "sz+x"
+  
+    have a3:"match_state1 (Next ?x xrs' xm' xss') (Next (?x + xpc) xrs' xm' xss')"
+      using a1 apply(unfold match_state1_def)
+      apply(cases "Next ?x xrs' xm' xss'",simp_all)
+      done
+  
+    (*hence a4:"match_state1 (x64_sem 1 l (Next x xrs xm xss)) (x64_sem 1 l_bin (Next (xpc+x) xrs xm xss))" sorry*)
+  
+    have "x64_sem num l_bin (Next (xpc+x) xrs xm xss) = fxst \<Longrightarrow> 
+    x64_sem num l (Next x xrs xm xss) = xxst \<Longrightarrow> 
+    list_in_list l xpc l_bin \<Longrightarrow> 
+    match_state1 xxst fxst" using Suc by simp
+  
+    have a5:"x64_sem num l_bin (Next (xpc+?x) xrs' xm' xss') = fxst" 
+      using a2 a1
+      by (metis Suc.prems(1) ab_semigroup_add_class.add_ac(1) add.commute b1 b2 plus_1_eq_Suc x64_sem_add) 
+    have a6:"x64_sem num l (Next ?x xrs' xm' xss') = xxst" using a1 a2
+      by (metis Suc.prems(2) add.commute d1 d2 plus_1_eq_Suc x64_sem_add) 
+    have "match_state1 xxst fxst" using a6 a5 assm2 Suc by blast
+    then show ?thesis by simp
+  next
+    case False
+    have "exec_instr ins sz (xpc+x) xrs xm xss = Stuck" using b1 False by simp
+    hence "exec_instr ins sz x xrs xm xss = Stuck" 
+      apply(unfold exec_instr_def)
+      apply(cases ins,simp_all)
+              subgoal for x7 apply(unfold exec_push_def Let_def)
+                apply(cases "storev M64 xm (Vptr sp_block (xrs (IR SP) - u64_of_memory_chunk M64)) (Vlong (xrs (IR x7)))",simp_all)
+                done
+              subgoal for x8 apply(unfold exec_pop_def Let_def)
+                apply(cases "loadv M64 xm (Vptr sp_block (xrs (IR SP)))",simp_all)
+                subgoal for a apply(cases a,simp_all)
+                  done
+                done
+              subgoal for x131 x132 apply(cases "eval_testcond x131 xrs",simp_all)
+                subgoal for a
+                  by (metis outcome.distinct(1))          
+                done
+              subgoal for x151 x152 x153
+                apply(unfold exec_store_def,simp_all)
+                apply(cases "storev x153 xm (Vlong (eval_addrmode64 x151 xrs)) (Vlong (xrs (IR x152)))",simp_all)
+                done
+              subgoal for x201 x202 x203 
+                apply(unfold exec_load_def,simp_all)
+                apply(cases "loadv x203 xm (Vlong (eval_addrmode64 x202 xrs))",simp_all)
+                subgoal for a apply(cases a,simp_all)
+                  done
+                done
+              subgoal for x21a 
+                apply(unfold exec_call_def,simp_all)
+                done
+              done
+    then show ?thesis using d2 by simp 
+  qed
+qed
+ 
 lemma one_step_equiv:
-  assumes a0:"flat_bpf_sem 1 (l_bin,l_pc,l_jump) (pc, xst) = fxst" and
+  assumes a0:"flat_bpf_sem 1 (l_bin,l_pc,l_jump) (pc, fxst) = fxst'" and
    a1:"jitflat_bpf lt init_second_layer = (l_bin,l_pc,l_jump)" and
-   a2:"perir_sem 1 lt (pc,xst) = xxst" and
-   a3:"xst = Next xpc xrs xm xss" and
-   a4:"lt \<noteq> []"
-  shows"fxst = xxst"
+   a2:"perir_sem 1 lt (pc,xxst) = xxst'" and
+   a3:"xxst = Next xpc xrs xm xss" and
+   a4:"lt \<noteq> []" and
+   a5:"match_state (pc, xxst) (pc, fxst)" and
+   a6:"snd xxst' \<noteq> Stuck" and
+   a7:"unat pc < length lt \<and> unat pc \<ge> 0"
+  shows"match_state xxst' fxst'"
 proof-
+  have "\<exists> xpc1. fxst = Next xpc1 xrs xm xss" using a3 a5 
+    apply(unfold match_state_def match_state1_def) 
+    apply(cases fxst,simp_all)
+    done
+  then obtain xpc1 where a6:"fxst = Next xpc1 xrs xm xss" by auto
+
   let "?curr_ins" = "lt!(unat pc)"
   let "?num" = "fst (lt!(unat pc))"
   let "?off" = "fst (snd (lt!(unat pc)))"
@@ -345,17 +551,15 @@ proof-
   let "?xpc" = "fst (l_pc ! (unat pc))"
   have c0:"list_in_list ?l (unat ?xpc) l_bin" 
     using flattern_l_bin0 init_second_layer_def a1 b0 a4 by (metis add_0 list.size(3)) 
-  have c1:"unat ?xpc= xpc" sorry
+  have c1:"unat ?xpc= xpc1" sorry
 
-
-
-  have "fxst = flat_bpf_one_step (l_bin,l_pc,l_jump) (pc, xst)" using a0
+  have "fxst' = flat_bpf_one_step (l_bin,l_pc,l_jump) (pc, Next xpc1 xrs xm xss)" using a0 a6
     by (metis One_nat_def flat_bpf_sem.simps(1) flat_bpf_sem.simps(2) old.prod.exhaust) 
-  hence c2:"fxst = (
+  hence c2:"fxst' = (
   let num = snd (l_pc!(unat pc)) in 
-        if l_bin!(xpc+1) = (0x39::u8) then \<comment>\<open> TODO: if the first byte is the opcode of cmp? \<close>
+        if l_bin!(xpc1+1) = (0x39::u8) then \<comment>\<open> TODO: if the first byte is the opcode of cmp? \<close>
           \<comment>\<open> case: BPF JMP \<close>
-          (case x64_sem 1 l_bin (Next xpc xrs xm xss) of
+          (case x64_sem 1 l_bin (Next xpc1 xrs xm xss) of
           Stuck \<Rightarrow> (pc, Stuck) | \<comment>\<open> if one step error, stop, it should be impossible \<close>
           Next xpc1 rs1 m1 ss1 \<Rightarrow> (
             if rs1 (CR ZF) = 1 then \<comment>\<open> must JUMP \<close>
@@ -364,21 +568,19 @@ proof-
               Some npc \<Rightarrow>
                 (npc, (Next (unat (fst (l_pc!(unat npc)))) rs1 m1 ss1))) \<comment>\<open> go to the target address in the jited x64 binary \<close>
             else \<comment>\<open> donot JUMP \<close>
-              (pc+1, xst)
+              (pc+1, fxst)
           ))
          else
           \<comment>\<open> case: NOT BPF JMP \<close>
-          (pc+1, x64_sem num l_bin (Next xpc xrs xm xss)))" 
+          (pc+1, x64_sem num l_bin (Next xpc1 xrs xm xss)))" 
     apply(unfold flat_bpf_one_step_def Let_def) 
-    using a3 apply(cases xst,simp_all)
-    subgoal for x11 by meson 
+    using a3 a6 apply(cases "Next xpc1 xrs xm xss",simp_all)
+    subgoal for x11 by meson  
     done
 
+  have "xxst' = perir_step lt (pc,xxst)" using a2 by (metis One_nat_def perir_sem.simps(1) perir_sem.simps(2) split_pairs)
 
-  have "xxst = perir_step lt (pc,xst)
-    " using a2 by (metis One_nat_def perir_sem.simps(1) perir_sem.simps(2) split_pairs)
-
-  hence b1:"xxst = (let (num,off,l) = lt!(unat pc) in 
+  hence b1:"xxst' = (let (num,off,l) = lt!(unat pc) in 
        if l!0 = 0xc3 then
           let (pc', ss', caller,fp) = update_stack2 xss in 
           let rs' = restore_x64_caller xrs caller fp in (pc', Next xpc rs' xm ss')
@@ -397,13 +599,13 @@ proof-
           Stuck \<Rightarrow> (pc, Stuck)      
       else
         let xst_temp = Next 0 xrs xm xss; xst' = x64_sem num l xst_temp in
-          (pc+1, xst'))" using perir_step_def b0 a2 a3 apply(cases xst,simp_all)
+          (pc+1, xst'))" using perir_step_def b0 a2 a3 apply(cases xxst,simp_all)
     done
 
   thus ?thesis
   proof(cases "?l!0 = 0xc3")
     case True
-    have "xxst = (let (num,off,l) = lt!(unat pc) in (let (pc', ss', caller,fp) = update_stack2 xss in 
+    have "xxst' = (let (num,off,l) = lt!(unat pc) in (let (pc', ss', caller,fp) = update_stack2 xss in 
           let rs' = restore_x64_caller xrs caller fp in (pc', Next xpc rs' xm ss')))"
       using b1 True by (smt (z3) b0 case_prod_conv)
     then show ?thesis sorry
@@ -414,7 +616,7 @@ proof-
     proof(cases "?l!0 = 0xe8")
       case True
       have b3:"?l!0 = 0xe8" using True by simp
-      have "xxst = (let caller = save_x64_caller xrs; fp = save_x64_frame_pointer xrs; 
+      have "xxst' = (let caller = save_x64_caller xrs; fp = save_x64_frame_pointer xrs; 
             rs' = upate_x64_stack_pointer xrs (stack_pointer xss) in
         let ss' = update_stack caller fp (pc+1) xss in
           (case ss' of None \<Rightarrow> (pc, Stuck) | 
@@ -427,7 +629,7 @@ proof-
       then show ?thesis
       proof(cases "?l!1 = (0x39::u8)")
         case True
-        hence "xxst = (let xst_temp = Next 0 xrs xm xss; xst' = x64_sem ?num ?l xst_temp in
+        hence "xxst' = (let xst_temp = Next 0 xrs xm xss; xst' = x64_sem ?num ?l xst_temp in
           case xst' of
           Next xpc' rs' m' ss'\<Rightarrow>
             if rs' (CR ZF) = 1 then (?off+pc, xst')
@@ -437,50 +639,42 @@ proof-
         then show ?thesis sorry
       next
         case False
-          have b6:"?l!0 \<noteq> 0xe8 \<and> ?l!0 \<noteq> 0xc3 \<and> ?l!1 \<noteq> (0x39::u8)" using b5 False by blast
-          have d0:"xxst = (let xst_temp = Next 0 xrs xm xss; xst' = x64_sem ?num ?l xst_temp in
+        have b6:"?l!0 \<noteq> 0xe8 \<and> ?l!0 \<noteq> 0xc3 \<and> ?l!1 \<noteq> (0x39::u8)" using b5 False by blast
+          have d0:"xxst' = (let xst_temp = Next 0 xrs xm xss; xst' = x64_sem ?num ?l xst_temp in
           (pc+1, xst'))" using b6 by (smt (verit) b0 b1 case_prod_conv)
           
-          have c3_0:"list_in_list ?l xpc l_bin" using c0 c1 by simp
+          have c3_0:"list_in_list ?l xpc1 l_bin" using c0 c1 by simp
           have c3_1:"?l \<noteq> []" sorry
-          have c3:"l_bin!xpc = ?l!0" using c3_0 c3_1
+          have c3:"l_bin!xpc1 = ?l!0" using c3_0 c3_1
             by (metis list_in_list.simps(2) list_in_list_prop neq_Nil_conv) 
            (* by (metis list.collapse list_in_list.simps(2)) *)
-          have c3_2:"l_bin!(xpc+1) \<noteq> (0x39::u8)" sorry
+          have c3_2:"l_bin!(xpc1+1) \<noteq> (0x39::u8)" sorry
           
-          have c4:"fxst = (let num = snd (l_pc!(unat pc)) in (pc+1, x64_sem num l_bin (Next xpc xrs xm xss)))"
-            using c2 c3 b6 c3_2 by auto
-          have c5_1:"l_pc \<noteq> []" sorry 
-          have c5:"fxst = (pc+1, x64_sem ?num l_bin (Next xpc xrs xm xss))"using flattern_num b0 c5_1 a1 init_second_layer_def c4
-            by (metis add_0 list.size(3)) 
-          have c6_1:"?num>0" sorry
-          have "x64_sem ?num l_bin (Next xpc xrs xm xss) = 
-              (case x64_decode xpc l_bin of
-                None \<Rightarrow> Stuck |
-                Some (sz, ins) \<Rightarrow>
-             x64_sem (?num-1) l_bin (exec_instr ins sz xpc xrs xm xss))" 
-            using c5 c6_1 by (metis Suc_diff_1 x64_sem.simps(3)) 
-          hence c6:"snd fxst = (case x64_decode xpc l_bin of
-                None \<Rightarrow> Stuck |
-                Some (sz, ins) \<Rightarrow>
-             x64_sem (?num-1) l_bin (exec_instr ins sz xpc xrs xm xss))"
-            by (simp add: c5) 
-          have d1:"snd xxst = 
-              (case x64_decode 0 ?l of
-                None \<Rightarrow> Stuck |
-                Some (sz, ins) \<Rightarrow>
-             x64_sem (?num-1) ?l (exec_instr ins sz 0 xrs xm xss))"
-            using d0 c6_1 by (metis Suc_diff_1 snd_conv x64_sem.simps(3)) 
-          have c7:"x64_decode 0 ?l = x64_decode xpc l_bin" 
-            using d1 c6 c0 c1 c3_1 list_in_list_prop2 by simp
-          have "snd fxst = snd xxst" using d1 c6 c0 c1 c7 sorry
-        then show ?thesis by (simp add: c5 d0) 
+          have c4:"fxst' = (let num = snd (l_pc!(unat pc)) in (pc+1, x64_sem num l_bin (Next xpc1 xrs xm xss)))"
+            using c2 c3 b6 c3_2 by presburger 
+          have c5_1:"l_pc \<noteq> []"  using a1 a4 apply(unfold init_second_layer_def) using num_corr by fastforce 
+
+          have c5:"fxst' = (pc+1, x64_sem ?num l_bin (Next xpc1 xrs xm xss))"using b0 c5_1 a1 init_second_layer_def c4 a6 a7
+            by (metis (mono_tags, lifting) flattern_num_easy)
+            
+
+          have cn:"match_state1 (snd xxst') (snd fxst')" using c5 d0 c3_0 list_in_list_prop3
+            by (metis add.right_neutral assms(7) snd_conv)
+            
+
+          have "fst fxst' = pc+1" using c5 by auto
+          moreover have d2:"fst xxst' = pc+1" using d0 by auto
+          hence "fst xxst' = fst fxst'" using calculation by presburger 
+          hence "match_state xxst' fxst'" using cn match_state_def match_state1_def 
+            apply(cases "snd xxst'",simp_all)
+            apply(cases "snd fxst'",simp_all)
+            by (simp add: case_prod_beta') 
+                   
+          then show ?thesis by (simp add: c5 d0) 
       qed
     qed
   qed
 qed
-  
-
 
 lemma flat_bpf_sem_induct_aux1:
  "flat_bpf_sem (m+n) x64_prog xst = xst'\<Longrightarrow> 
@@ -512,51 +706,65 @@ lemma intermediate_step_is_ok:"perir_sem n lt (pc,s) = s' \<Longrightarrow> n \<
   apply simp 
   using err_is_still_err
   apply (meson outcome.exhaust)
-  by (metis JITFlattern.err_is_still_err outcome.exhaust prod.collapse)  
+  by (metis JITFlattern.err_is_still_err outcome.exhaust prod.collapse) 
 
 
 lemma n_steps_equiv:
-  "flat_bpf_sem n prog xst = fxst \<Longrightarrow>
+  "flat_bpf_sem n prog (pc,fxst) = fxst' \<Longrightarrow>
   jitflat_bpf lt init_second_layer = prog \<Longrightarrow>
-  perir_sem n lt xst = xxst \<Longrightarrow>
-  snd xst = Next xpc xrs xm xss \<Longrightarrow>
-  snd xxst = Next xpc' xrs' xm' xss' \<Longrightarrow>
-  lt \<noteq> [] \<Longrightarrow>
-  fxst = xxst"
-proof(induct n arbitrary: prog xst fxst lt xxst xpc xrs xm xss xpc' xrs' xm' xss')
+  perir_sem n lt (pc,xxst) = xxst' \<Longrightarrow>
+  xxst = Next xpc xrs xm xss \<Longrightarrow>
+  snd xxst' = Next xpc' xrs' xm' xss' \<Longrightarrow>
+  match_state (pc,xxst) (pc,fxst) \<Longrightarrow>
+  lt \<noteq> [] \<Longrightarrow> 
+  unat pc < length lt \<and> unat pc \<ge> 0 \<Longrightarrow>
+  match_state xxst' fxst'"
+proof(induct n arbitrary: prog pc fxst fxst' lt xxst xxst' xpc xrs xm xss xxst' xpc' xrs' xm' xss')
   case 0
-  then show ?case by (metis flat_bpf_sem.simps(1) perir_sem.simps(1) prod.collapse)
+  then show ?case apply(unfold match_state_def,simp_all) 
+    done
     
 next
   case (Suc n)
-  assume assm0:"flat_bpf_sem (Suc n) prog xst = fxst" and 
+  assume assm0:"flat_bpf_sem (Suc n) prog (pc,fxst) = fxst'" and 
   assm1:"jitflat_bpf lt init_second_layer = prog" and
-  assm2:"perir_sem (Suc n) lt xst = xxst" and
-  assm3:"snd xst = Next xpc xrs xm xss" and
-  assm4:"snd xxst = Next xpc' xrs' xm' xss'" and
-  assm5:"lt \<noteq> []"
-  have "\<exists> next_s. next_s = perir_sem 1 lt xst" by simp
-  then obtain next_s where b0:"next_s = perir_sem 1 lt xst" by auto
-  have "\<exists> next_f. flat_bpf_sem 1 prog xst = next_f" by blast
-  then obtain next_f where b1:"flat_bpf_sem 1 prog xst = next_f" by simp
-  have bn:"next_s = next_f" using assm1 b0 b1 assm3 one_step_equiv assm5
-    by (metis prod.collapse)
-  have a0:"perir_sem n lt next_s = xxst" using x64_sem1_induct_aux3 assm2 b0 by blast
-  have "\<exists> xrs1 xpc1 m1 xss1. snd next_s = Next xrs1 xpc1 m1 xss1" using assm4 a0 intermediate_step_is_ok a0 
-    by (metis bot_nat_0.extremum outcome.distinct(1) prod.collapse)
-  then obtain xrs1 xpc1 m1 xss1 where a1:"snd next_s = Next xrs1 xpc1 m1 xss1" by auto
-
-  have c0:"flat_bpf_sem n prog next_f = fxst" using flat_bpf_sem_induct_aux2 assm0 b1 by blast
-  have c1:"snd next_f = Next xrs1 xpc1 m1 xss1" using a1 bn b0 by blast
+  assm2:"perir_sem (Suc n) lt (pc,xxst) = xxst'" and
+  assm3:"xxst = Next xpc xrs xm xss" and
+  assm4:"snd xxst' = Next xpc' xrs' xm' xss'" and
+  assm5:"lt \<noteq> []" and
+  assm6:"match_state (pc,xxst) (pc,fxst)" and
+  assm7:"unat pc < length lt \<and> unat pc \<ge> 0"
+  have "\<exists> next_s. next_s = perir_sem 1 lt (pc,xxst)" by simp
+  then obtain next_s pc' where b0:"next_s = perir_sem 1 lt (pc,xxst)" by auto
+  have "\<exists> next_f. flat_bpf_sem 1 prog (pc,fxst) = next_f" by blast
+  then obtain next_f where b1:"flat_bpf_sem 1 prog (pc,fxst) = next_f" by simp
+  (*have b2:"xrs1 = xrs \<and> xm = xm1 \<and> xss = xss1" using match_state_def assm3 assm7 assm6
+    apply(cases "fxst",simp_all)
+    done*)
+  have a0:"perir_sem n lt next_s = xxst'" using x64_sem1_induct_aux3 assm2 b0
+    using Suc.prems(3) by presburger 
+  have "\<exists> pc' xrs1 xpc1 m1 xss1. (pc', Next xrs1 xpc1 m1 xss1) = next_s" using assm4 a0 intermediate_step_is_ok a0
+    by (metis outcome.exhaust prod.collapse zero_le) 
+  then obtain pc' xrs1 xpc1 m1 xss1 where a1:"(pc', Next xrs1 xpc1 m1 xss1) = next_s" by auto
   
-  have "flat_bpf_sem n prog xst = fxst \<Longrightarrow>
-    jitflat_bpf lt init_second_layer = prog \<Longrightarrow> 
-    perir_sem n lt xst = xxst \<Longrightarrow> 
-    snd xst = Next xpc xrs xm xss \<Longrightarrow> 
-    fxst = xxst" using Suc by blast
-  have "fxst = xxst" using a0 a1 c1 c1 Suc bn c0 by blast 
+  have bn:"match_state next_s next_f"
+    using one_step_equiv b1 assm1 b0 assm3 assm5 assm6 a1 assm7 by (metis eq_snd_iff outcome.distinct(1)) 
+
+  have a2:"(pc', snd next_f) = next_f" using bn match_state_def a1 b0 b1
+    apply(cases "Next xrs1 xpc1 m1 xss1",simp_all)
+    apply(cases "snd next_f",simp_all)
+    subgoal for x11 x11a x12 x13 x14 by force
+    subgoal for x11 by force
+    done
+
+  have c0:"flat_bpf_sem n prog next_f = fxst'" using flat_bpf_sem_induct_aux2 assm0 b1 by blast
+
+  have "unat pc' < length lt \<and> unat pc \<ge> 0" sorry
+  hence "match_state xxst' fxst'" 
+    using a0 a1 a2 Suc bn c0 assm5 assm4 assm7 by (metis bot_nat_0.extremum) 
   then show ?case by simp
 qed
+
 
 
 end
